notation change

LambdaLetDollar.v
@@ -43,14 +43,14 @@ Definition non_to_tm' {A} (p : non' A) :=
 Coercion non_to_tm' : non' >-> tm'.
 
 Declare Custom Entry λ_let_dollar_scope.
-Notation "<{ e }>'" := e (at level 1, e custom λ_let_dollar_scope at level 99).
+Notation "<| e |>" := e (at level 1, e custom λ_let_dollar_scope at level 99).
 Notation "( x )" := x (in custom λ_let_dollar_scope, x at level 99).
 Notation "{ x }" := x (in custom λ_let_dollar_scope at level 0, x constr).
 Notation "x" := x (in custom λ_let_dollar_scope at level 0, x constr at level 0).
 Notation "'var' v" := (tm_var' v) (in custom λ_let_dollar_scope at level 1, left associativity).
-Notation "0" := <{ var None }>' (in custom λ_let_dollar_scope at level 0).
-Notation "1" := <{ var {Some None} }>' (in custom λ_let_dollar_scope at level 0).
-Notation "2" := <{ var {Some (Some None)} }>' (in custom λ_let_dollar_scope at level 0).
+Notation "0" := <| var None |> (in custom λ_let_dollar_scope at level 0).
+Notation "1" := <| var {Some None} |> (in custom λ_let_dollar_scope at level 0).
+Notation "2" := <| var {Some (Some None)} |> (in custom λ_let_dollar_scope at level 0).
 Notation "'λ' e" := (tm_abs' e)
     (in custom λ_let_dollar_scope at level 90,
       e custom λ_let_dollar_scope at level 99,
@@ -70,12 +70,12 @@ Notation "'let' e1 'in' e2" := (tm_let' e1 e2) (in custom λ_let_dollar_scope at
 
 Fixpoint map' {A B : Type} (f : A -> B) (e : tm' A) : tm' B :=
   match e with
-  | <{ var a }>' => <{ var {f a} }>'
-  | <{ λ  e' }>' => <{ λ  {map' (option_map f) e'} }>'
-  | <{ S₀ e' }>' => <{ S₀ {map' (option_map f) e'} }>'
-  | <{ e1   e2 }>' => <{ {map' f e1}   {map' f e2} }>'
-  | <{ e1 $ e2 }>' => <{ {map' f e1} $ {map' f e2} }>'
-  | <{ let e1 in e2 }>' => tm_let' (map' f e1) (map' (option_map f) e2)
+  | <| var a |> => <| var {f a} |>
+  | <| λ  e' |> => <| λ  {map' (option_map f) e'} |>
+  | <| S₀ e' |> => <| S₀ {map' (option_map f) e'} |>
+  | <| e1   e2 |> => <| {map' f e1}   {map' f e2} |>
+  | <| e1 $ e2 |> => <| {map' f e1} $ {map' f e2} |>
+  | <| let e1 in e2 |> => tm_let' (map' f e1) (map' (option_map f) e2)
   end.
 
 (* Lemma map_id_law : forall {V} (f : V -> V) e,
@@ -89,20 +89,20 @@ Admitted. *)
 
 Fixpoint bind' {A B : Type} (f : A -> tm' B) (e : tm' A) : tm' B :=
   match e with
-  | <{ var a }>' => f a
-  | <{ e1   e2 }>' => <{ {bind' f e1}   {bind' f e2} }>'
-  | <{ e1 $ e2 }>' => <{ {bind' f e1} $ {bind' f e2} }>'
-  | <{ λ  e' }>' => tm_abs' (bind' (fun a' => 
+  | <| var a |> => f a
+  | <| e1   e2 |> => <| {bind' f e1}   {bind' f e2} |>
+  | <| e1 $ e2 |> => <| {bind' f e1} $ {bind' f e2} |>
+  | <| λ  e' |> => tm_abs' (bind' (fun a' => 
       match a' with
       | None   => tm_var' None
       | Some a => map' Some (f a)
       end) e')
-  | <{ S₀ e' }>' => tm_s_0' (bind' (fun a' => 
+  | <| S₀ e' |> => tm_s_0' (bind' (fun a' => 
       match a' with
       | None   => tm_var' None
       | Some a => map' Some (f a)
       end) e')
-  | <{ let e1 in e2 }>' => tm_let' (bind' f e1) (bind' (fun a' => 
+  | <| let e1 in e2 |> => tm_let' (bind' f e1) (bind' (fun a' => 
       match a' with
       | None   => tm_var' None
       | Some a => map' Some (f a)
@@ -121,7 +121,7 @@ Admitted. *)
 Definition var_subst' {V} e' (v:^V) :=
   match v with
   | None => e'
-  | Some v => <{ var v }>'
+  | Some v => <| var v |>
   end.
 
 Definition tm_subst0' {V} (e:tm' ^V) (v:val' V) :=
@@ -142,12 +142,12 @@ Notation "E [ e ]" := (plug' E e)
 
 Definition tm_dec' (e : tm' ␀) : (val' ␀ + non' ␀) :=
   match e with
-  | <{ var a }>' => from_void a
-  | <{ λ  e' }>' => inl (val_abs' e')
-  | <{ S₀ e' }>' => inr (non_s_0' e')
-  | <{ e1   e2 }>' => inr (non_app' e1 e2)
-  | <{ e1 $ e2 }>' => inr (non_dol' e1 e2)
-  | <{ let e1 in e2 }>' => inr (non_let' e1 e2)
+  | <| var a |> => from_void a
+  | <| λ  e' |> => inl (val_abs' e')
+  | <| S₀ e' |> => inr (non_s_0' e')
+  | <| e1   e2 |> => inr (non_app' e1 e2)
+  | <| e1 $ e2 |> => inr (non_dol' e1 e2)
+  | <| let e1 in e2 |> => inr (non_let' e1 e2)
   end.
 Lemma tm_dec_val' : ∀ e v, tm_dec' e = inl v → e = val_to_tm' v.
 Proof.
@@ -227,51 +227,51 @@ Arguments dec' A : clear implicits.
 
 Definition plugJ' {A} (j : J' A) e' :=
   match j with
-  | J_fun' e => <{ e' e }>'
-  | J_arg' v => <{ v  e' }>'
-  | J_dol' e => <{ e' $ e }>'
+  | J_fun' e => <| e' e |>
+  | J_arg' v => <| v  e' |>
+  | J_dol' e => <| e' $ e |>
   end.
 Instance PlugJ' : Plug' J' := @plugJ'.
 
 Fixpoint plugK' {A} (k : K' A) e :=
   match k with
   | K_nil' => e
-  | K_let' k1 e2 => <{ let {plugK' k1 e} in e2 }>'
+  | K_let' k1 e2 => <| let {plugK' k1 e} in e2 |>
   end.
 Instance PlugK' : Plug' K' := @plugK'.
 
 Fixpoint plugT' {A} (trail : T' A) e :=
   match trail with
   | T_nil' => e
-  | T_cons' v k t => <{ v $ k [{plugT' t e}] }>'
+  | T_cons' v k t => <| v $ k [{plugT' t e}] |>
   end.
 Instance PlugT' : Plug' T' := @plugT'.
 
 Definition redex_to_term' {A} (r : redex' A) := 
   match r with
-  | redex_beta'   v1 v2 => <{ v1 v2 }>'
-  | redex_dollar' v1 v2 => <{ v1 $ v2 }>'
-  | redex_shift'  v  e  => <{ v $ S₀ e }>'
-  | redex_dol_let' v e1 e2 => <{ v $ let S₀ e1 in e2 }>'
-  | redex_let' j p  => <{ j[p] }>'
-  | redex_let_beta' v e => <{ let v in e }>'
-  | redex_let_assoc' e1 e2 e3 => <{ let (let S₀ e1 in e2) in e3 }>'
+  | redex_beta'   v1 v2 => <| v1 v2 |>
+  | redex_dollar' v1 v2 => <| v1 $ v2 |>
+  | redex_shift'  v  e  => <| v $ S₀ e |>
+  | redex_dol_let' v e1 e2 => <| v $ let S₀ e1 in e2 |>
+  | redex_let' j p  => <| j[p] |>
+  | redex_let_beta' v e => <| let v in e |>
+  | redex_let_assoc' e1 e2 e3 => <| let (let S₀ e1 in e2) in e3 |>
   end.
 Coercion redex_to_term' : redex' >-> tm'.
 
 Definition stuck_to_non' : tm' ^␀ * option (tm' ^␀) → non' ␀ := λ s,
   match s with
   | (e, None) => non_s_0' e
-  | (e1, Some e2) => non_let' <{ S₀ e1 }>' e2
+  | (e1, Some e2) => non_let' <| S₀ e1 |> e2
   end.
 
 
 Fixpoint decompose' (e : tm' ␀) : dec' ␀ :=
   match e with
-  | <{ var a }>' => from_void a
-  | <{ λ  e' }>' => dec_value' (val_abs' e')
-  | <{ S₀ e' }>' => dec_stuck_s_0' e'
-  | <{ e1 e2 }>' =>
+  | <| var a |> => from_void a
+  | <| λ  e' |> => dec_value' (val_abs' e')
+  | <| S₀ e' |> => dec_stuck_s_0' e'
+  | <| e1 e2 |> =>
     match tm_dec' e1 with
     | inr p1 => dec_redex' K_nil' T_nil' (redex_let' (J_fun' e2) p1) (* p1 e2 *)
     | inl v1 =>
@@ -280,7 +280,7 @@ Fixpoint decompose' (e : tm' ␀) : dec' ␀ :=
       | inl v2 => dec_redex' K_nil' T_nil' (redex_beta' v1 v2)         (* v1 v2 *)
       end
     end
-  | <{ e1 $ e2 }>' =>
+  | <| e1 $ e2 |> =>
     match tm_dec' e1 with
     | inr p1 => dec_redex' K_nil' T_nil' (redex_let' (J_dol' e2) p1) (* p1 $ e2 *)
     | inl v1 => (* v1 $ e *)
@@ -291,7 +291,7 @@ Fixpoint decompose' (e : tm' ␀) : dec' ␀ :=
       | dec_value' v2            => dec_redex' K_nil' (T_nil')         (redex_dollar' v1 v2)         (* v1 $ v2 *)
       end
     end
-  | <{ let e1 in e2 }>' =>
+  | <| let e1 in e2 |> =>
     match decompose' e1 with
     | dec_stuck_s_0' e1'       => dec_stuck_let' e1' e2                                           (* let x = S₀ f. e1' in e2 *)
     | dec_stuck_let' e1_1 e1_2 => dec_redex' (K_nil')      T_nil' (redex_let_assoc' e1_1 e1_2 e2) (* let x = (let y = S₀ f. e1_1 in e1_2) in e2 *)
@@ -345,14 +345,14 @@ Proof.
   - inv_decompose_match' H.
 Qed.
 Lemma decompose_stuck_s_0_inversion' : ∀ e e',
-  decompose' e = dec_stuck_s_0' e' → e = <{ S₀ e' }>'.
+  decompose' e = dec_stuck_s_0' e' → e = <| S₀ e' |>.
 Proof.
   intros. inv e; cbn in *; reason;
   try solve [inversion a | inv H];
   inv_decompose_match' H.
 Qed.
 Lemma decompose_stuck_let_inversion' : ∀ e e' e'',
-  decompose' e = dec_stuck_let' e' e'' → e = <{ let S₀ e' in e'' }>'.
+  decompose' e = dec_stuck_let' e' e'' → e = <| let S₀ e' in e'' |>.
 Proof.
   intros. inv e; cbn in *; reason;
   try solve [inversion a | inv H];
@@ -366,7 +366,7 @@ Ltac inv_dec' :=
   | H : dec_stuck_let' ?e1 ?e2 = decompose' ?e |- _ => rewrite (decompose_stuck_let_inversion' e e1 e2); cbn; auto
   end.
 Lemma decompose_redex_inversion' : ∀ e t k r,
-  decompose' e = dec_redex' k t r → e = <{ k[t[r]] }>'.
+  decompose' e = dec_redex' k t r → e = <| k[t[r]] |>.
 Proof.
   dependent induction e; intros; cbn in *; reason;
   try solve [destruct a | inv H];
@@ -382,17 +382,17 @@ Proof.
   intros; destruct v; auto.
 Qed.
 Lemma decompose_plug_stuck_s_0' : ∀ e, 
-  decompose' <{ S₀ e }>' = dec_stuck_s_0' e.
+  decompose' <| S₀ e |> = dec_stuck_s_0' e.
 Proof.
   auto.
 Qed.
 Lemma decompose_plug_stuck_let' : ∀ e1 e2,
-  decompose' <{ let S₀ e1 in e2 }>' = dec_stuck_let' e1 e2.
+  decompose' <| let S₀ e1 in e2 |> = dec_stuck_let' e1 e2.
 Proof.
   auto.
 Qed.
 Lemma decompose_plug_redex' : ∀ k t (r : redex' ␀),
-  decompose' <{ k[t[r]] }>' = dec_redex' k t r.
+  decompose' <| k[t[r]] |> = dec_redex' k t r.
 Proof with cbn; auto.
   intros k t; generalize dependent k; induction t; intros...
   - induction k...
@@ -432,31 +432,31 @@ Instance LiftK' : Lift K' := @liftK'.
 Definition contract' (r : redex' ␀) : tm' ␀ :=
   match r with
   (* (λ x. e) v  ~>  e [x := v] *)
-  | redex_beta' (val_abs' e) v => <{ e [0 := v] }>'
+  | redex_beta' (val_abs' e) v => <| e [0 := v] |>
 
   (* v1 $ v2  ~>  v1 v2 *)
-  | redex_dollar' v1 v2 => <{ v1 v2 }>'
+  | redex_dollar' v1 v2 => <| v1 v2 |>
 
   (* v $ S₀ f. e  ~>  e [f := λ x. v $ x] *)
-  | redex_shift' v e  => <{ e [0 := v] }>'
-  (* | redex_shift' v e  => <{ e [0 := λv' {liftV' v} $ 0] }>' *)
+  | redex_shift' v e  => <| e [0 := v] |>
+  (* | redex_shift' v e  => <| e [0 := λv' {liftV' v} $ 0] |> *)
 
   (* v $ let x = S₀ f. e1 in e2  ~>  (λ x. v $ e2) $ S₀ f. e1 *)
-  | redex_dol_let' v e1 e2 => <{ (λ {liftV' v} $ e2) $ S₀ e1 }>'
+  | redex_dol_let' v e1 e2 => <| (λ {liftV' v} $ e2) $ S₀ e1 |>
 
   (* J[p]  ~>  let x = p in J[x] *)
-  | redex_let' j p => <{ let p in ↑j[0] }>'
+  | redex_let' j p => <| let p in ↑j[0] |>
 
   (* let x = v in e  ~>  e [x := v] *)
-  | redex_let_beta' v e => <{ e [0 := v] }>'
+  | redex_let_beta' v e => <| e [0 := v] |>
 
   (* let x = (let y = S₀ f. e1 in e2) in e3  ~>  let y = S₀ f. e1 in let x = e2 in e3*)
-  | redex_let_assoc' e1 e2 e3 => <{ let S₀ e1 in let e2 in ↑e3 }>'
+  | redex_let_assoc' e1 e2 e3 => <| let S₀ e1 in let e2 in ↑e3 |>
   end.
 
 Definition optional_step' e :=
   match decompose' e with
-  | dec_redex' k t r => Some <{ k[t[{contract' r}]] }>'
+  | dec_redex' k t r => Some <| k[t[{contract' r}]] |>
   | _ => None
   end.
 
@@ -468,7 +468,7 @@ Global Hint Constructors contr' : core.
 
 Reserved Notation "e1 -->' e2" (at level 40).
 Inductive step' : tm' ␀ → tm' ␀ → Prop :=
-| step_tm' : ∀ k t e1 e2, <{ k[t[e1]] }>' -->' <{ k[t[e2]] }>'
+| step_tm' : ∀ k t e1 e2, <| k[t[e1]] |> -->' <| k[t[e2]] |>
 where "e1 -->' e2" := (step' e1 e2).
 
 Notation "e1 -->'* e2" := (multi step' e1 e2) (at level 40).
@@ -484,47 +484,47 @@ Fixpoint eval' i e :=
   end.
 
 Section Examples.
-  Definition _id : tm' ␀ := <{ λ 0 }>'.
-  Definition _const : tm' ␀ := <{ λ λ 1 }>'.
+  Definition _id : tm' ␀ := <| λ 0 |>.
+  Definition _const : tm' ␀ := <| λ λ 1 |>.
 
-  Compute (eval' 10 <{ _id $ _const $ S₀ 0 }>').
-  Compute (eval' 10 <{ _const $ _id $ S₀ 0 }>').
+  Compute (eval' 10 <| _id $ _const $ S₀ 0 |>).
+  Compute (eval' 10 <| _const $ _id $ S₀ 0 |>).
 
-  Definition j1 : J' ␀ := J_fun' <{ λ 0 0 }>'.
-  Definition j2 : J' ␀ := J_arg' <{ λv' 0 }>'.
-  Definition j3 : J' ␀ := J_dol' <{ λ 0 }>'.
-  Definition ej123 := <{ j1[j2[j3[S₀ 0]]] }>'.
+  Definition j1 : J' ␀ := J_fun' <| λ 0 0 |>.
+  Definition j2 : J' ␀ := J_arg' <| λv' 0 |>.
+  Definition j3 : J' ␀ := J_dol' <| λ 0 |>.
+  Definition ej123 := <| j1[j2[j3[S₀ 0]]] |>.
 
-  Example from_K_to_K' : eval' 3 ej123 = <{ 
+  Example from_K_to_K' : eval' 3 ej123 = <| 
     let
       let
         let S₀ 0
         in ↑j3[0]
       in ↑j2[0]
     in ↑j1[0]
-  }>'. Proof. auto. Qed.
+  |>. Proof. auto. Qed.
 
-  Example from_K_to_stuck' : eval' 5 ej123 = <{ 
+  Example from_K_to_stuck' : eval' 5 ej123 = <| 
     let S₀ 0 in
     let
       let ↑j3[0]
       in ↑↑j2[1]
     in ↑↑j1[1]
-  }>'. Proof. auto. Qed.
+  |>. Proof. auto. Qed.
 
-  Example ex_dol_let : eval' 6 <{ _id $ ej123 }>' = <{ 
+  Example ex_dol_let : eval' 6 <| _id $ ej123 |> = <| 
     (λ ↑_id $ 
       let
         let ↑j3[0]
         in ↑↑j2[1]
       in ↑↑j1[1]
     ) $ S₀ 0
-  }>'. Proof. cbn. auto. Qed.
+  |>. Proof. cbn. auto. Qed.
 
-  Example ex_shift : eval' 7 <{ _id $ ej123 }>' = <{
+  Example ex_shift : eval' 7 <| _id $ ej123 |> = <|
     λ ↑_id $ let (let ↑j3[0] in ↑↑j2[1]) in ↑↑j1[1]
-  }>'. Proof. cbn. auto. Qed.
+  |>. Proof. cbn. auto. Qed.
 
-  Compute (decompose' (eval' 7 <{ _id $ ej123 }>')).
+  Compute (decompose' (eval' 7 <| _id $ ej123 |>)).
   
 End Examples.
